src/Actus/Types/Automata.lean
@@ -67,6 +67,26 @@ def GuardCondition.eval (gc : GuardCondition) (clockValues : ClockMap) : Bool :=
 def GuardConditions.eval (gcs : GuardConditions) (clockValues : ClockMap) : Bool :=
   gcs.conditions.all (fun gc => gc.eval clockValues)
 
+inductive Alternation {α : Type} : Type where
+| tru : Alternation
+| fls : Alternation
+| and : Alternation → Alternation → Alternation
+| or : Alternation → Alternation → Alternation
+| var : α → Alternation
+| cond : GuardCondition -> Alternation
+| reset_in : ClockVar -> Alternation -> Alternation
+  deriving BEq, Hashable, Repr
+
+-- to lift this from one-clock, we probably replace the `v` indexing the `|=` with a `ClockMap`. This would be a breaking change.
+inductive Alternation.Eval {α : Type} (M : α × Clock) : ClockMap -> @Alternation α -> Prop where
+| tru : forall v, Alternation.Eval M v Alternation.tru
+| and : forall v a b, Alternation.Eval M v a -> Alternation.Eval M v b -> Alternation.Eval M v (Alternation.and a b)
+| or_left : forall v a b, Alternation.Eval M v a -> Alternation.Eval M v (Alternation.or a b)
+| or_right : forall v a b, Alternation.Eval M v b -> Alternation.Eval M v (Alternation.or a b)
+| var : forall (v : ClockMap), v.toList.contains ({name:=0}, M.2) -> Alternation.Eval M v (Alternation.var M.1)
+| cond : forall v (gc : GuardCondition), (exists (cv : ClockMap), gc.eval cv = true) -> Alternation.Eval M v (Alternation.cond gc)
+| reset_in : forall v, Alternation.Eval M (Lean.AssocList.empty.insert {name:=0} {tick:=0}) a -> Alternation.Eval M v (Alternation.reset_in { name := 0 } a)
+
 namespace Execution
   structure Entry where
     state : State
